Example.lean
@@ -1,0 +1,222 @@
+import Init.Meta
+import Parser
+import Lemmas
+
+open Lean Lean.Syntax Parser Parser.Char
+
+/- Example for howto transform a partial parser into a total parser -/
+
+/-- -/
+abbrev TestParser := SimpleParser String.Slice Char
+
+/-- -/
+inductive Ast where
+| pure : Char → Ast
+| cons : Char → Ast → Ast
+deriving Repr, Inhabited
+
+instance : ToString Ast :=
+  let rec pp : Ast → String
+  | .pure e => toString e
+  | .cons e es => toString e ++ " | " ++ pp es
+  ⟨pp⟩
+
+/-- -/
+def digit : TestParser Char :=
+  withErrorMessage "<digit>" do
+    tokenMap fun c => if c >= '0' && c <= '9' then some c else none
+
+/-- -/
+def bar : TestParser Char :=
+  withErrorMessage "<bar>" do
+    tokenMap fun c => if c = '|' then some c else none
+
+/-- -/
+def digitBar : TestParser Char := do
+    let d ← digit
+    bar *> return d
+
+namespace Theorems
+
+theorem digitRespectsPositionOnOk (h : digit it = Result.ok s a)
+    : Stream.RespectsPosition.respectsPosition Char it s := by
+  have : respectsPosition _ _ digit := by simp [digit]
+  simp [respectsPosition] at this
+  grind [this it (by solve_by_elim)]
+
+theorem digitRespectsPositionOnError (h : digit it = Result.error s e)
+    : Stream.RespectsPosition.respectsPosition Char it s := by
+  have : respectsPosition _ _ digit := by simp [digit]
+  simp [respectsPosition] at this
+  grind [this it (by solve_by_elim)]
+
+@[simp] theorem digitBarRespectsPosition
+    : respectsPosition _ _ digitBar := by
+  simp [digitBar, bind, respectsPosition]
+  intro it hv
+  split
+  · rename_i heq
+    split at heq
+    · expose_names
+      have h2 : Stream.RespectsPosition.respectsPosition Char s rem := by
+        have := seqRightRespectsPosition _ _ bar (pure a_1) (by simp [bar]) (by simp)
+        simp [respectsPosition] at this
+        grind [this s (by assumption)]
+      exact Stream.RespectsPosition.isEquivalence.trans (digitRespectsPositionOnOk heq_1) h2
+    · simp_all
+  · expose_names
+    split at heq
+    · expose_names
+      have h2 : Stream.RespectsPosition.respectsPosition Char s rem := by
+        have := seqRightRespectsPosition _ _ bar (pure a_1) (by simp [bar]) (by simp)
+        simp [respectsPosition] at this
+        grind [this s (by assumption)]
+      exact Stream.RespectsPosition.isEquivalence.trans (digitRespectsPositionOnOk heq_1) h2
+    · expose_names
+      have := digitRespectsPositionOnError heq_1
+      simp [pure] at heq
+      grind
+
+@[simp] theorem digitBarDecrementsRemainingOnSuccess
+    : decrementsRemainingOnSuccess _ _ digitBar := by
+  simp [digitBar, bind, decrementsRemainingOnSuccess]
+  intro it rem a hv h
+  generalize "<ast>: expected digit" = txt at h
+  split at h
+  · rename_i s a_1 heq
+    have h1 : Stream.decrementsRemaining it s := by
+      have : decrementsRemainingOnSuccess _ _ digit := by simp [digit]
+      simp [decrementsRemainingOnSuccess] at this
+      grind
+    have h2 : Stream.notIncrementsRemaining s rem := by
+      have := seqRightNotIncrementsRemainingOnSuccess _ _ bar (pure a_1) (by simp [bar]) (by simp)
+      simp [notIncrementsRemainingOnSuccess] at this
+      exact this s rem a (by assumption) (by assumption)
+    simp [Stream.decrementsRemaining] at h1
+    simp [Stream.notIncrementsRemaining] at h2
+    grind [Stream.decrementsRemaining]
+  · simp_all
+
+end Theorems
+
+/-- -/
+def mkSimpleError (it : String.Slice) (msg : String)
+    : Parser.Result (Error.Simple String.Slice Char) String.Slice α :=
+  .error it (Error.Simple.addMessage
+    (Error.Simple.unexpected it.startInclusive.offset none) it.startInclusive.offset msg)
+
+/-- -/
+def run (p : TestParser Ast) (input : String) : IO Unit :=
+  match p.run input.toSlice with
+  | .ok rem x => IO.println s!"ok {x}, remaining chars {rem.chars.length}"
+  | .error rem e => IO.println s!"error {e} at pos {rem.startInclusive.offset}"
+
+namespace Test1
+
+/-- partial function -/
+partial def ast : TestParser Ast := do
+  let d ← digit
+  Ast.cons d <$> (bar *> ast) <|> return Ast.pure d
+
+/--
+info: ok 1 | 2, remaining chars 0
+-/
+#guard_msgs in
+#eval run ast "1|2"
+
+end Test1
+
+namespace Test2
+
+open Parser.Stream in
+/--
+  The recursive function ``loop`` calls ``p`` with a parser that acts like ``p``
+  except it fails if called from the same or lower string position
+
+  see https://leanprover.zulipchat.com/#narrow/channel/113488-general/topic/Advent.20of.20Code.3F/near/405471085
+-/
+def loop (p : SimpleParser String.Slice Char α → SimpleParser String.Slice Char α)
+    : SimpleParser String.Slice Char α := fun it =>
+  let p' : SimpleParser String.Slice Char α := fun it' =>
+    if Remaining.remaining it' < Remaining.remaining it then
+      loop p it'
+    else
+      return mkSimpleError it' "recursive call going backwards in the string"
+  p p' it
+termination_by it => Remaining.remaining it
+
+/-- prove termination  at runtime  -/
+def ast : TestParser Ast :=
+  loop fun p => do
+    let d ← digit
+    Ast.cons d <$> (bar *> p) <|> return Ast.pure d
+
+/--
+info: ok 1 | 2, remaining chars 0
+-/
+#guard_msgs in
+#eval run ast "1|2"
+
+end Test2
+
+namespace Test3
+
+/-- -/
+partial def ast : TestParser Ast :=
+    (digitBar >>= fun d => ast >>= fun a => pure (Ast.cons d a))
+    <|> (do let d ← digit; pure (Ast.pure d))
+
+/--
+info: ok 1 | 2 | 3, remaining chars 0
+-/
+#guard_msgs in
+#eval run ast "1|2|3"
+
+end Test3
+
+namespace Test4
+
+open Parser.Stream in
+/-- loop corresponds to the following parser:
+```
+  loop := (do let x ← pre; post x <$> loop) <|> alternative
+```
+or
+```
+  loop := (pre >>= fun x => loop >>= fun y => post x y) <|> alternative
+```
+  with the property ```Parser.decrementsRemainingOnSuccess pre```
+  which proves termination
+-/
+def loop
+  (pre : SimpleParser String.Slice Char β)
+  (post : β → α → SimpleParser String.Slice Char α)
+  (alternative : SimpleParser String.Slice Char α)
+  (h : decrementsRemainingOnSuccess _ _ pre)
+    : SimpleParser String.Slice Char α := fun it =>
+  match hm : pre it with
+  | .ok it' b =>
+      have := ltRemainingOfDecrementsRemainingOnSuccess pre hm (by solve_by_elim) h
+      match loop pre post alternative h it' with
+      | .ok it'' a =>
+        match post b a it'' with
+        | .ok rem a => .ok rem a
+        | .error _ _ => alternative it
+      | .error _ _ => alternative it
+  | .error _ _ => alternative it
+termination_by it => Remaining.remaining it
+
+/-- prove termination at compile time  -/
+def ast : TestParser Ast :=
+    loop
+      digitBar (fun d rest => pure (Ast.cons d rest))
+      /- <|> -/ (do let d ← digit; pure (Ast.pure d))
+      (by simp)
+
+/--
+info: ok 1 | 2 | 3, remaining chars 0
+-/
+#guard_msgs in
+#eval run ast "1|2|3"
+
+end Test4
